AEAD packaging (WIP)

src/tls/AEAD.Pkg.fst
@@ -1,105 +1,249 @@
+(**
+  This modules packages AEAD.fsti as a "local package" and provides
+  a functor for constructing an AEAD package from an index package
+
+  TODO:
+  The next step is to restore AEADProvider using a compile-time flag to multiplex
+  between the 3 different providers: Low (verified), LowC (verification lost in translation)
+  and OpenSSL. This compile-time flag is such that ~Low ==> ~model
+  (we only idealize if the provider is Low).
+
+  TODO:
+  As a verification unit-test, we may show how to package two
+  instances of AEAD (for both directions) from the same create/coerce
+  on their concatenated keys, in TLS 1.2 style.
+*)
 module AEAD.Pkg
-
-// TODO instead: package from a plausible AEAD.fsti, mirroring
-// SecureAPI's one with bytes instead of buffers.
-
-// As a second step, we will restore AEADProvider between the two, and
-// use it to switch to faster, concrete, correct implementations.
-
-// As a verification unit-test, we may also show how to package two
-// instances of AEAD (for both directions) from the same create/coerce
-// on their concatenated keys, in tLS 1.2 style.
 
 open Mem
 open Pkg
 
 module HH = FStar.HyperHeap // I wish we could avoid it once Mem is open.
 
-/// --------------------------------------------------------------------------------------------------
-/// module AEAD
-/// sample generic, agile functionality.
-///
-/// TODO package instead StAE; what to do with the algorithm?
+module AE = AEAD
+module I  = Crypto.Indexing
 
-type aeadAlg = | AES_GCM128 | AES_GCM256
-let aeadLen: aeadAlg -> keylen = function
+/// TODO package instead StAE? what to do with the algorithm?
+
+type aeadAlg =
+  | AES_GCM128
+  | AES_GCM256
+
+val ideal: b:bool{b ==> model}
+let ideal =
+  assume (Flags.ideal_AEAD ==> model);
+  Flags.ideal_AEAD
+
+type safe (#ip:ipkg) (i:ip.t) = ideal /\ ip.honest i
+
+private val is_safe: #ip:ipkg -> i:ip.t{ip.registered i} -> ST bool
+  (requires fun _ -> True)
+  (ensures  fun h0 b h1 -> modifies_none h0 h1 /\ (b <==> safe i))
+let is_safe #ip i =
+  let honest = ip.get_honesty i in
+  ideal && honest
+
+type info = {
+  parent: r:rgn{~(is_tls_rgn r)};
+  alg: aeadAlg
+}
+
+type info1 (#ip:ipkg) (aeadAlg_of_i:ip.t -> aeadAlg) (i:ip.t) =
+  u:info{u.alg == aeadAlg_of_i i}
+
+val keylen: aeadAlg -> keylen
+let keylen = function
   | AES_GCM128 -> 32ul
   | AES_GCM256 -> 48ul
 
-// 17-10-31  this abbreviation breaks typechecking when used; why?
-// unfold type aeadAlgi (#ip:ipkg aeadAlg) (i:ip.t) = a:aeadAlg {a == ip.get_info i}
+type keyrepr (u:info) = lbytes (keylen u.alg)
 
-assume val flag_AEAD: b:bool{b ==> model}
-type idealAEAD = b2t flag_AEAD
+noeq abstract type concrete_key =
+  | AEAD: u:info -> k:keyrepr u -> concrete_key
 
-type keyrepr a = lbytes (aeadLen a)
-assume new type key (ip: ipkg) (aeadAlg_of_i: ip.t -> aeadAlg) (i:ip.t{ip.registered i}) // abstraction required for indexing
+noeq abstract type _key (#ip:ipkg) (index_of_i:ip.t -> I.id) (i:ip.t) =
+  | Ideal:
+    ck: concrete_key ->
+//    region: subrgn ck.u.parent{~(is_tls_rgn region)} ->
+    state: AE.aead_state (index_of_i i) I.Writer ->
+    _key #ip index_of_i i
+  | Real:
+    ck: concrete_key -> _key #ip index_of_i i
 
-let prf_region: subrgn tls_tables_region = new_region tls_tables_region
+type key (ip:ipkg)
+  (index_of_i:ip.t -> I.id)
+  (i:ip.t{ip.registered i}) =
+  (if model then
+    k:_key index_of_i i{Ideal? k <==> safe i}
+  else
+    concrete_key)
 
-let aead_shared_footprint (#ip:ipkg) (#aeadAlg_of_i: ip.t -> aeadAlg) : rset =
-  assume false; // Downward closed
-  Set.singleton prf_region
+val usage:
+  #ip:ipkg ->
+  #index_of_i:(ip.t -> I.id) ->
+  #i:ip.t{ip.registered i} ->
+  k:key ip index_of_i i ->
+  GTot info
+let usage #ip #index_of_i #i k =
+  if model then
+    match k <: _key index_of_i i with
+    | Ideal ck _ -> ck.u
+    | Real ck -> ck.u
+  else k.u
 
-assume val aead_footprint:
-  #ip:ipkg -> #aeadAlg_of_i: (ip.t -> aeadAlg) -> #i:ip.t{ip.registered i} ->
-  k:key ip aeadAlg_of_i i -> GTot (s:rset{s `Set.disjoint` aead_shared_footprint #ip #aeadAlg_of_i})
+val keyval:
+  #ip:ipkg ->
+  #index_of_i:(ip.t -> I.id) ->
+  #i:ip.t{ip.registered i} ->
+  k:key ip index_of_i i ->
+  GTot (keyrepr (usage k))
+let keyval #ip #index_of_i #i k =
+  if model then
+    match k <: _key index_of_i i with
+    | Ideal ck _ -> ck.k
+    | Real ck -> ck.k
+  else k.k
 
-// The local AEAD invariant
-assume val aead_inv:
-  #ip:ipkg -> #aeadAlg_of_i: (ip.t -> aeadAlg) -> #i:ip.t{ip.registered i} ->
-  k:key ip aeadAlg_of_i i -> h:mem -> GTot Type0
+(** Downward closure of [prf_region i] *)
+val shared_footprint:
+  #ip:ipkg ->
+  index_of_i:(ip.t -> I.id) ->
+  i:ip.t{ip.registered i} ->
+  GTot rset
+let shared_footprint #ip index_of_i i =
+  if model then AE.shared_footprint (index_of_i i)
+  else Set.empty
 
-assume val aead_invariant_framing: ip:ipkg -> aeadAlg_of_i: (ip.t -> aeadAlg) ->
-  i:ip.t{ip.registered i} -> k:key ip aeadAlg_of_i i ->
-  h0:mem -> r:HH.rid -> h1:mem ->
-  Lemma (requires aead_inv k h0 /\ modifies_one r h0 h1
-          /\ ~(r `Set.mem` aead_footprint k) /\ ~(r `Set.mem` aead_shared_footprint #ip #aeadAlg_of_i))
-        (ensures aead_inv k h1)
+val footprint:
+  #ip:ipkg ->
+  #index_of_i:(ip.t -> I.id) ->
+  #i:ip.t{ip.registered i} ->
+  k:key ip index_of_i i ->
+  GTot (s:rset{s `Set.disjoint` shared_footprint index_of_i i})
+let footprint #ip #index_of_i #i k =
+  Set.lemma_equal_intro (Set.empty `Set.intersect` shared_footprint index_of_i i) Set.empty;
+  if model then
+    match k <: _key index_of_i i with
+    | Ideal _ st -> AE.footprint st
+    | Real _ -> Set.empty
+  else Set.empty
 
-assume val aead_empty_log: ip: ipkg -> aeadAlg_of_i: (ip.t -> aeadAlg) ->
-  #i: ip.t{ip.registered i} -> a: aeadAlg {a == aeadAlg_of_i i} ->
-  k:key ip aeadAlg_of_i i -> h1:mem -> Type0
+(** The local AEAD invariant *)
+val invariant:
+  #ip:ipkg ->
+  #index_of_i:(ip.t -> I.id) ->
+  #i:ip.t{ip.registered i} ->
+  k:key ip index_of_i i ->
+  h:mem ->
+  GTot Type0
+let invariant #ip #index_of_i #i k h =
+  if model then
+    match k <: _key index_of_i i with
+    | Ideal _ st -> AE.invariant st h
+    | Real _ -> True
+  else True
 
-assume val aead_empty_log_framing: ip: ipkg -> aeadAlg_of_i: (ip.t -> aeadAlg) ->
-  #i: ip.t{ip.registered i} -> a: aeadAlg {a == aeadAlg_of_i i} ->
-  k:key ip aeadAlg_of_i i -> h0:mem -> r:HH.rid -> h1:mem -> Lemma
-    (requires (aead_empty_log ip aeadAlg_of_i a k h0 /\ modifies_one r h0 h1 /\ ~(r `Set.mem` aead_footprint k)))
-    (ensures (aead_empty_log ip aeadAlg_of_i a k h1))
+val invariant_framing:
+  #ip:ipkg ->
+  #index_of_i:(ip.t -> I.id) ->
+  #i:ip.t{ip.registered i} ->
+  k:key ip index_of_i i ->
+  h0:mem ->
+  r:HH.rid ->
+  h1:mem ->
+  Lemma (requires invariant k h0 /\
+         modifies_one r h0 h1 /\
+         ~(r `Set.mem` footprint k) /\
+         ~(r `Set.mem` shared_footprint index_of_i i))
+        (ensures invariant k h1)
+let invariant_framing #ip #index_of_i #i k h0 r h1 =
+  if model then
+    match k <: _key index_of_i i with
+    | Ideal _ st -> AE.frame_invariant st h0 r h1
+    | Real _ -> ()
 
-assume val create_key: ip: ipkg -> aeadAlg_of_i: (ip.t -> aeadAlg) ->
-  i: ip.t{ip.registered i} -> a:aeadAlg {a == aeadAlg_of_i i} ->
-  ST (key ip aeadAlg_of_i i)
-    (requires fun h0 -> model)
-    (ensures fun h0 k h1 -> modifies_none h0 h1 /\ fresh_regions (aead_footprint k) h0 h1
-      /\ aead_empty_log ip aeadAlg_of_i a k h1 /\ aead_inv k h1)
+val empty_log:
+  #ip:ipkg ->
+  #aeadAlg_of_i:(ip.t -> aeadAlg) ->
+  #index_of_i:(ip.t -> I.id) ->
+  #i:ip.t{ip.registered i} ->
+  a:aeadAlg{a == aeadAlg_of_i i} ->
+  k:key ip aeadAlg_of_i index_of_i i ->
+  h:mem ->
+  GTot Type0
+let empty_log #ip #aeadAlg_of_i #index_of_i #i a k h =
+  if AE.safeMac (index_of_i i) then AE.log k h == Seq.createEmpty else True
 
-assume val coerceT_key: ip: ipkg -> aeadAlg_of_i: (ip.t -> aeadAlg) ->
-  i: ip.t{ip.registered i /\ (idealAEAD ==> ~(ip.honest i))} ->
-  a:aeadAlg {a == aeadAlg_of_i i} -> keyrepr a ->
+val empty_log_framing:
+  #ip:ipkg ->
+  #aeadAlg_of_i:(ip.t -> aeadAlg) ->
+  #index_of_i:(ip.t -> I.id) ->
+  #i:ip.t{ip.registered i} ->
+  a:aeadAlg{a == aeadAlg_of_i i} ->
+  k:key ip aeadAlg_of_i index_of_i i ->
+  h0:mem ->
+  r:HH.rid ->
+  h1:mem ->
+  Lemma
+    (requires (empty_log a k h0 /\
+               modifies_one r h0 h1 /\
+               ~(r `Set.mem` footprint k)))
+    (ensures  (empty_log a k h1))
+let empty_log_framing #ip #aeadAlg_of_i #index_of_i #i a k h0 r h1 =
+  if AE.safeMac (index_of_i i) then AE.frame_log k Seq.createEmpty h0 r h1
+
+val create_key:
+  ip:ipkg ->
+  aeadAlg_of_i:(ip.t -> aeadAlg) ->
+  index_of_i:(ip.t -> I.id) ->
+  i:ip.t{ip.registered i} ->
+  a:aeadAlg{a == aeadAlg_of_i i} ->
+  ST (key ip aeadAlg_of_i index_of_i i)
+     (requires fun h0 -> model /\ live_region h0 (AE.prf_region (index_of_i i)))
+     (ensures  fun h0 k h1 ->
+       modifies_none h0 h1 /\
+       fresh_regions (footprint k) h0 h1 /\
+       empty_log a k h1 /\
+       invariant k h1)
+let create_key ip aeadAlg_of_i index_of_i i a =
+  let id = index_of_i i in
+  let log_rgn = new_region tls_tables_region in
+  AE.gen id (AE.prf_region id) log_rgn
+
+val coerceT_key:
+  ip:ipkg ->
+  aeadAlg_of_i:(ip.t -> aeadAlg) ->
+  index_of_i:(ip.t -> I.id) ->
+  i:ip.t{ip.registered i /\ (idealAEAD ==> ~(ip.honest i))} ->
+  a:aeadAlg{a == aeadAlg_of_i i} ->
+  keyrepr a ->
   GTot (key ip aeadAlg_of_i i)
 
-assume val coerce_key: ip: ipkg -> aeadAlg_of_i: (ip.t -> aeadAlg) ->
-  i: ip.t{ip.registered i /\ (idealAEAD ==> ~(ip.honest i))} ->
-  a:aeadAlg {a == aeadAlg_of_i i} -> k0:keyrepr a ->
+
+assume val coerce_key:
+  ip:ipkg ->
+  aeadAlg_of_i:(ip.t -> aeadAlg) ->
+  i:ip.t{ip.registered i /\ (idealAEAD ==> ~(ip.honest i))} ->
+  a:aeadAlg {a == aeadAlg_of_i i} ->
+  k0:keyrepr a ->
   ST (key ip aeadAlg_of_i i)
     (requires fun h0 -> True)
     (ensures fun h0 k h1 -> k == coerceT_key ip aeadAlg_of_i i a k0
       /\ modifies_none h0 h1 /\ fresh_regions (aead_footprint k) h0 h1
-      /\ aead_empty_log ip aeadAlg_of_i a k h1 /\ aead_inv k h1)
+      /\ aead_empty_log ip aeadAlg_of_i a k h1 /\ invariant k h1)
 
-let local_ae_pkg (ip:ipkg) (aeadAlg_of_i: ip.t -> aeadAlg) =
+let local_ae_pkg (ip:ipkg) (aeadAlg_of_i:ip.t -> aeadAlg) =
   LocalPkg
     (key ip aeadAlg_of_i)
-    (fun (i:ip.t) -> a:aeadAlg{a = aeadAlg_of_i i})
-    (fun #_ a -> aeadLen a)
+    (info aeadAlg_of_i)
+    keylen
     idealAEAD
-    (aead_shared_footprint #ip #aeadAlg_of_i)
-    (aead_footprint #ip #aeadAlg_of_i)
-    (aead_inv #ip #aeadAlg_of_i)
-    (aead_invariant_framing ip aeadAlg_of_i)
-    (aead_empty_log ip aeadAlg_of_i)
-    (aead_empty_log_framing ip aeadAlg_of_i)
+    (shared_footprint #ip #aeadAlg_of_i)
+    (footprint #ip #aeadAlg_of_i)
+    (invariant #ip #aeadAlg_of_i)
+    (invariant_framing ip aeadAlg_of_i)
+    (empty_log ip aeadAlg_of_i)
+    (empty_log_framing ip aeadAlg_of_i)
     (create_key ip aeadAlg_of_i)
     (coerceT_key ip aeadAlg_of_i)
     (coerce_key ip aeadAlg_of_i)
@@ -116,9 +260,8 @@ let mp (ip:ipkg) (aeadAlg_of_i: ip.t -> aeadAlg): ST (pkg ip)
 val encrypt:
   ip:ipkg -> aeadAlg_of_i: (ip.t -> aeadAlg) -> #i:ip.t{ip.registered i} ->
   k: key ip aeadAlg_of_i i -> nat -> ST nat
-  (requires fun h0 -> aead_inv k h0)
+  (requires fun h0 -> invariant k h0)
   (ensures fun h0 c h1 ->
-    modifies (rset_union (aead_footprint k) (aead_shared_footprint #ip #aeadAlg_of_i)) h0 h1
-    /\ aead_inv k h1)
-
+    modifies (rset_union (footprint k) (shared_footprint #ip #aeadAlg_of_i)) h0 h1
+    /\ invariant k h1)
 let encrypt _ _ #_ k v = v + 1
