src/tls/AEAD.fsti
@@ -1,0 +1,281 @@
+(**
+  This interfaces provides an abstraction for the verfieid Hacl* Crypto.AEAD.Main module,
+  using Platform.Bytes rather than buffers.
+*)
+module AEAD
+
+module I = Crypto.Indexing
+module HH = FStar.HyperHeap
+module U32 = FStar.UInt32
+module U128 = FStar.UInt128
+module Plain = Crypto.Plain
+
+open FStar.UInt32
+open Mem
+open Pkg
+
+let ivlen (alg:I.cipherAlg) = 12ul
+
+let taglen = 16ul
+
+let iv (alg:I.cipherAlg) =
+  let open FStar.Mul in
+  n:U128.t { U128.v n < pow2 (8 * v (ivlen alg)) }
+
+let aadmax =
+  assert_norm (2000 <= pow2 32 - 1);
+  2000ul // arbitrary; enough for TLS
+
+type aadlen_32 = l:U32.t {l <=^ aadmax}
+
+val keylen   : I.id -> U32.t
+
+val statelen : I.id -> U32.t
+
+type cipher (i:I.id) (l:nat{l + v taglen < pow2 32}) = lbytes (uint_to_t l +^ taglen)
+
+inline_for_extraction
+val entry : i:I.id -> Type0
+
+let nonce (i:I.id) = iv (I.cipherAlg_of_id i)
+
+type adata = b:bytes{Seq.length b <= v aadmax}
+
+type plainLen = l:Plain.plainLen{l + v taglen < pow2 32}
+
+val mk_entry (#i:I.id) :
+    nonce:nonce i ->
+    ad:adata ->
+    #l:plainLen ->
+    p:Plain.plain i l ->
+    c:cipher i (Seq.length (Plain.as_bytes p)) ->
+    entry i
+
+val entry_injective (#i:I.id)
+                    (n:nonce i) (n':nonce i)
+                    (ad:adata) (ad':adata)
+                    (#l:plainLen) (#l':plainLen)
+                    (p:Plain.plain i l) (p':Plain.plain i l')
+                    (c:cipher i (Seq.length (Plain.as_bytes p))) (c':cipher i (Seq.length (Plain.as_bytes p')))
+  : Lemma (let e  = mk_entry n ad p c in
+           let e' = mk_entry n' ad' p' c' in
+           (e == e' <==> (n == n' /\ ad == ad' /\ l == l' /\ p == p' /\ c == c')))
+
+val nonce_of_entry (#i:_) (e:entry i) : nonce i
+
+let safeMac (i:I.id) = Flag.safeHS i && Flag.mac1 i
+
+let safeId  (i:I.id) = Flag.safeId i
+
+val aead_state: I.id -> I.rw -> Type0
+
+val log_region: #i:_ -> #rw:_ -> aead_state i rw -> subrgn tls_tables_region
+
+val prf_region: i:I.id -> subrgn tls_tables_region
+
+val log: #i:_ -> #rw:_ -> s:aead_state i rw{safeMac i} -> mem -> GTot (Seq.seq (entry i))
+
+let address = nat
+
+let addr_unused_in (rid:HH.rid) (a:address) (m0:mem) =
+  Monotonic.Heap.addr_unused_in a (Map.sel m0.h rid)
+
+let contains_addr (rid:HH.rid) (a:address) (m:mem) =
+  ~(addr_unused_in rid a m)
+
+let fresh_addresses (rid:HH.rid) (addrs:Set.set address) (m0:mem) (m1:mem) =
+  forall a. a `Set.mem` addrs ==>
+       addr_unused_in rid a m0 /\
+       contains_addr  rid a m1
+
+(** Downward closure of [prf_region i] *)
+val shared_footprint: i:I.id -> GTot rset
+
+(** Downward closure of [log_region i] *)
+val footprint: #i:I.id -> #rw:_ -> aead_state i rw -> 
+  GTot (s:rset{s `Set.disjoint` shared_footprint i})
+
+//Leaving this abstract for now; but it should imply Crypto.AEAD.Invariant.safelen i len (otp_offset i)
+val safelen: I.id -> nat -> bool
+
+let ok_plain_len_32 (i:I.id) = l:U32.t{safelen i (v l)}
+
+val invariant : #i:_ -> #rw:_ -> aead_state i rw -> mem -> Type0
+
+val frame_invariant: #i:_ -> #rw:_ -> st:aead_state i rw -> h0:mem -> r:HH.rid -> h1:mem ->
+    Lemma (requires (invariant st h0 /\
+           modifies_one r h0 h1 /\
+           ~(r `Set.mem` footprint st) /\
+           ~(r `Set.mem` shared_footprint i)))
+          (ensures invariant st h1)
+
+val frame_log: #i:_ -> #rw:_ -> st:aead_state i rw -> l:Seq.seq (entry i) ->
+  h0:mem -> r:HH.rid -> h1:mem ->
+  Lemma (requires
+          safeMac i /\
+          log st h0 == l /\
+          modifies_one r h0 h1 /\
+          ~(r `Set.mem` footprint st))
+        (ensures log st h1 == l)
+
+(*** The main stateful API ***)
+
+(** Allocating a writer **)
+val gen (i:I.id)
+        (prf_rgn:subrgn tls_tables_region)
+        (log_rgn:subrgn tls_tables_region)
+  : ST (aead_state i I.Writer)
+    (requires (fun h -> prf_rgn `HH.disjoint` log_rgn))
+    (ensures  (fun h0 s h1 ->
+               log_region s == log_rgn /\
+               prf_region i == prf_rgn /\
+               modifies_none h0 h1 /\ // allocates only
+               (exists fresh.
+                  fresh_addresses prf_rgn fresh h0 h1 /\
+                  footprint s == Set.singleton log_rgn /\
+                  shared_footprint i == Set.singleton prf_rgn) /\
+               (safeMac i ==> log s h1 == Seq.createEmpty) /\
+               invariant s h1
+              ))
+
+(*
+(** Building a reader from a writer **)
+(* A reader never writes to the log_region, but may write to the prf_region *)
+let read_footprint (#i:_) (wr:aead_state i I.Writer) : GTot fp =
+  FStar.TSet.filter (fun (rs:(HH.rid * refs_in_region)) -> fst rs == prf_region wr)
+                    (footprint wr)
+
+val genReader
+           (#i: I.id)
+           (wr: aead_state i I.Writer)
+ : ST (aead_state i I.Reader)
+  (requires (fun h -> invariant wr h))
+  (ensures  (fun h0 rd h1 ->
+               HS.modifies Set.empty h0 h1 /\
+               invariant rd h1 /\
+               log_region rd == log_region wr /\
+               prf_region rd == prf_region wr /\
+               footprint  rd == read_footprint wr))
+
+
+(** [coerce]: Only needed for modeling the adversary *)
+val coerce
+         (i: I.id)
+       (rgn: eternal_region)
+       (key: lbuffer (v (keylen i)))
+      : ST  (aead_state i I.Writer)
+  (requires (fun h ->
+             ~ (Flag.prf i) /\
+             Buffer.live h key))
+  (ensures  (fun h0 st h1 ->
+               HS.modifies Set.empty h0 h1 /\
+               invariant st h1))
+
+(** [leak]: Only needed for modeling the adversary *)
+val leak
+      (#i: I.id)
+      (st: aead_state i I.Writer)
+    : ST (lbuffer (v (statelen i)))
+  (requires (fun _ -> ~(Flag.prf i)))
+  (ensures  (fun h0 _ h1 ->
+               HS.modifies Set.empty h0 h1 /\
+               invariant st h1))
+
+// enc_dec_separation: Calling AEAD.encrypt/decrypt requires this separation
+let enc_dec_separation (#i:_) (#rw:_) (st:aead_state i rw)
+                       (#aadlen:nat) (aad: lbuffer aadlen)
+                       (#plainlen:nat) (plain: Plain.plainBuffer i plainlen)
+                       (#cipherlen: nat) (cipher:lbuffer cipherlen) =
+    Buffer.disjoint aad cipher /\
+    Buffer.disjoint (Plain.as_buffer plain) aad /\
+    Buffer.disjoint (Plain.as_buffer plain) cipher /\
+    HH.disjoint_regions (Set.as_set [Buffer.frameOf (Plain.as_buffer plain);
+                                     Buffer.frameOf cipher;
+                                     Buffer.frameOf aad])
+                        (Set.as_set [log_region st;
+                                     prf_region st]) /\
+    Buffer.frameOf cipher <> HH.root /\
+    Buffer.frameOf aad <> HH.root /\
+    Buffer.frameOf (Plain.as_buffer plain) <> HH.root
+    (* HS.is_eternal_region (Buffer.frameOf cipher) /\ // why? *)
+    (* HS.is_eternal_region (Buffer.frameOf (Plain.as_buffer plain)) /\ //why? *)
+    (* HS.is_eternal_region (Buffer.frameOf aad) /\ //why? *)
+
+let enc_dec_liveness (#i:_) (#rw:_) (st:aead_state i rw)
+                     (#aadlen:nat) (aad: lbuffer aadlen)
+                     (#plainlen:nat) (plain: Plain.plainBuffer i plainlen)
+                     (#cipherlen: nat) (cipher:lbuffer cipherlen) (h:mem) =
+    let open HS in
+    Buffer.live h aad /\
+    Buffer.live h cipher /\
+    Plain.live h plain /\
+    log_region st `is_in` h.h /\
+    prf_region st `is_in` h.h
+
+let entry_of
+          (#i: I.id)
+           (n: iv (I.cipherAlg_of_id i))
+     (#aadlen: aadlen_32)
+         (aad: lbuffer (v aadlen))
+   (#plainlen: ok_plain_len_32 i)
+       (plain: Plain.plainBuffer i (v plainlen))
+  (cipher_tag: lbuffer (v plainlen + v taglen))
+           (h: mem) : GTot (entry i) =
+  let aad = Buffer.as_seq h aad in
+  let p = Plain.sel_plain h plainlen plain in
+  let c = Buffer.as_seq h cipher_tag in
+  mk_entry n aad p c
+
+let entry_for_nonce (#i:_) (#rw:_) (n:nonce i) (st:aead_state i rw) (h:mem{safeMac i})
+  : GTot (option (entry i)) =
+    Seq.find_l (fun e -> nonce_of_entry e = n) (log st h)
+
+let fresh_nonce (#i:_) (#rw:_) (n:nonce i) (st:aead_state i rw) (h:mem{safeMac i}): GTot bool =
+  None? (entry_for_nonce n st h)
+
+let just_one_buffer (#a:Type) (b:Buffer.buffer a) : GTot fp =
+   as_set [(Buffer.frameOf b, SomeRefs (as_set [Buffer.as_addr b]))]
+
+val encrypt
+          (i: I.id)
+         (st: aead_state i I.Writer)
+          (n: iv (I.cipherAlg_of_id i))
+     (aadlen: aadlen_32)
+        (aad: lbuffer (v aadlen))
+   (plainlen: ok_plain_len_32 i)
+      (plain: Plain.plainBuffer i (v plainlen))
+ (cipher_tag: lbuffer (v plainlen + v taglen))
+            : ST unit
+  (requires (fun h ->
+               enc_dec_separation st aad plain cipher_tag /\
+               enc_dec_liveness st aad plain cipher_tag h /\
+               invariant st h /\
+               (safeMac i ==> fresh_nonce n st h)))
+  (ensures (fun h0 _ h1 ->
+               modifies_fp (footprint st `TSet.union` just_one_buffer cipher_tag) h0 h1 /\
+               enc_dec_liveness st aad plain cipher_tag h1 /\
+               invariant st h1 /\
+               (safeMac i ==>
+                   log st h1 ==
+                   Seq.snoc (log st h0) (entry_of n aad plain cipher_tag h1))))
+
+val decrypt
+          (i: I.id)
+         (st: aead_state i I.Reader)
+          (n: iv (I.cipherAlg_of_id i))
+     (aadlen: aadlen_32)
+        (aad: lbuffer (v aadlen))
+   (plainlen: ok_plain_len_32 i)
+      (plain: Plain.plainBuffer i (v plainlen))
+ (cipher_tag: lbuffer (v plainlen + v taglen))
+            : ST bool
+  (requires (fun h ->
+               enc_dec_separation st aad plain cipher_tag /\
+               enc_dec_liveness st aad plain cipher_tag h /\
+               invariant st h))
+  (ensures (fun h0 verified h1 ->
+               invariant st h1 /\
+               enc_dec_liveness st aad plain cipher_tag h1 /\
+               modifies_fp (footprint st `TSet.union` just_one_buffer (Plain.as_buffer plain)) h0 h1 /\
+               (safeId i ==> entry_for_nonce n st h1 == Some (entry_of n aad plain cipher_tag h1))))
+*)
