src/tls/IV.fst
@@ -23,46 +23,50 @@ let sample (len:UInt32.t): ST (lbytes len)
 
 // should be set together with its parent KDF.
 assume val flag_Raw: b:bool{b ==> model}
+
 type idealRaw = b2t flag_Raw
 
-type rawlen (#ip: ipkg) (#len_of_i: ip.t -> keylen) (i:ip.t) = len:keylen {len = len_of_i i}
-type raw (ip: ipkg) (len_of_i: ip.t -> keylen) (i:ip.t{ip.registered i}) = lbytes (len_of_i i)
+// SZ: [len_of_i] was implicit, but it can't be inferred from [i]. Made it explicit
+type rawlen (#ip:ipkg) (len_of_i:ip.t -> keylen) (i:ip.t) = len:keylen {len == len_of_i i}
 
-let shared_footprint_raw (ip: ipkg) (len_of_i: ip.t -> keylen): rset = Set.empty
+type raw (ip:ipkg) (len_of_i:ip.t -> keylen) (i:ip.t{ip.registered i}) = lbytes (len_of_i i)
 
-let footprint_raw (ip: ipkg) (len_of_i: ip.t -> keylen)
+let shared_footprint_raw (ip:ipkg) (len_of_i:ip.t -> keylen): rset = Set.empty
+
+let footprint_raw (ip:ipkg) (len_of_i:ip.t -> keylen)
   (#i:ip.t {ip.registered i}) (k:raw ip len_of_i i)
   : GTot (s:rset{s `Set.disjoint` shared_footprint_raw ip len_of_i})
   =
   let fp = Set.empty in
-  assume(fp `Set.disjoint` shared_footprint_raw ip len_of_i);
+  let sfp = shared_footprint_raw ip len_of_i in
+  Set.lemma_equal_elim (fp `Set.intersect` sfp) Set.empty;
   fp
 
-let create_raw (ip: ipkg) (len_of_i: ip.t -> keylen)
+let create_raw (ip:ipkg) (len_of_i:ip.t -> keylen)
   (i:ip.t{ip.registered i}) (len:keylen {len = len_of_i i}):
   ST (raw ip len_of_i i)
   (requires fun h0 -> model)
   (ensures fun h0 p h1 -> modifies_none h0 h1)
   = sample len
 
-let coerceT_raw (ip: ipkg) (len_of_i: ip.t -> keylen)
+let coerceT_raw (ip:ipkg) (len_of_i:ip.t -> keylen)
   (i: ip.t {ip.registered i /\ (idealRaw ==> ~(ip.honest i))})
-  (len:keylen {len = len_of_i i}) (r:lbytes len):
+  (len:keylen{len == len_of_i i}) (r:lbytes len):
   GTot (raw ip len_of_i i) = r
 
 let coerce_raw (ip: ipkg) (len_of_i: ip.t -> keylen)
   (i: ip.t {ip.registered i /\ (idealRaw ==> ~(ip.honest i))})
-  (len:keylen {len = len_of_i i}) (r:lbytes len):
+  (len:keylen {len == len_of_i i}) (r:lbytes len):
   ST (raw ip len_of_i i)
   (requires fun h0 -> True)
   (ensures fun h0 k h1 -> k == coerceT_raw ip len_of_i i len r /\ modifies_none h0 h1)
   = r
 
-let local_raw_pkg (ip:ipkg) (len_of_i: ip.t -> keylen) : local_pkg ip =
+let local_raw_pkg (ip:ipkg) (len_of_i:ip.t -> keylen) : local_pkg ip =
   LocalPkg
     (raw ip len_of_i)
-    (rawlen #ip #len_of_i)
-    (fun #i (n:rawlen i) -> n)
+    (rawlen #ip len_of_i)
+    (fun #i (n:rawlen len_of_i i) -> n)
     idealRaw
     (shared_footprint_raw ip len_of_i)
     (footprint_raw ip len_of_i)
@@ -74,7 +78,7 @@ let local_raw_pkg (ip:ipkg) (len_of_i: ip.t -> keylen) : local_pkg ip =
     (coerceT_raw ip len_of_i)
     (coerce_raw ip len_of_i)
 
-let rp (ip:ipkg) (len_of_i: ip.t -> keylen): ST (pkg ip)
+let rp (ip:ipkg) (len_of_i:ip.t -> keylen): ST (pkg ip)
   (requires fun h0 -> True)
   (ensures fun h0 p h1 -> modifies_one tls_define_region h0 h1 /\ p.package_invariant h1)
   =
